forward convertion proof

sppf/sppf.v
@@ -1,12 +1,23 @@
 Import Nat.
 
+Require Import fl.cfg.Definitions.
+Require Import fl.int.Base2.
+Require Import fl.cfg.Derivation.
+
 Require Import List.
 
 Module Base.
-
   Import ListNotations.
 
+  Import Definitions Derivation.
+  Import Base2.Base.
+
   Context {Tt Vt: Type}.
+
+  Inductive ext_der {Tt Vt} (G : (@grammar Tt Vt)) : (list symbol) -> (list symbol) -> Prop :=
+    | refl (p : list symbol) : ext_der G p p
+    | inDer A p (in_der : (der G A p)): ext_der G [Vs A] p.
+
 
   Inductive SPPF_node : Type :=
   | mk_terminal_node : Tt  -> nat -> nat -> SPPF_node
@@ -30,31 +41,32 @@ Module Base.
   Inductive sppf_der (sppf: SPPF) :  SPPF_node -> word -> Prop :=
   |  terDer (t : Tt) (from : nat) (to : nat) : sppf_der sppf (mk_terminal_node t from to) [T t]
   |  epsilonDer (from : nat) (to : nat) : sppf_der sppf (mk_epsilon_node from to) []
-  |  mkRel1 p vp ch1 w1 : In (mk_rel p vp (mk_packed_node1 ch1)) sppf ->
+  |  mkRel1 p (vp : valid_parent p) ch1 w1 : In (mk_rel vp (mk_packed_node1 ch1)) sppf ->
                           (sppf_der sppf ch1 w1) -> sppf_der sppf p w1
-  |  mkRel2 p vp ch1 ch2 w1 w2 : In (mk_rel p vp (mk_packed_node2 ch1 ch2)) sppf ->
-                                 (sppf_der sppf ch1 w1) -> (sppf_der sppf ch2 w2) -> sppf_der sppf p w1.
+  |  mkRel2 p (vp : valid_parent p) ch1 ch2 w1 w2 : In (mk_rel vp (mk_packed_node2 ch1 ch2)) sppf ->
+                                 (sppf_der sppf ch1 w1) -> (sppf_der sppf ch2 w2) -> sppf_der sppf p (w1 ++ w2).
 
   Inductive triple :=
-    mkTriple : nat -> (@phrase Tt Vt) -> nat -> triple.
+  |  var_triple : nat -> Vt -> nat -> triple
+  |  phrase_triple : nat -> (@phrase Tt Vt) -> nat -> triple.
 
   Definition valid_parent_to_triple (s : SPPF_node) (vp : (valid_parent s)) : triple  :=
     match vp with
-    | mk_nonterminal_node_parent v from to => (mkTriple from [Vs (V v)] to)
-    | mk_intermediate_node_parent p from to => (mkTriple from p to)
+    | mk_nonterminal_node_parent v from to => (var_triple from v to)
+    | mk_intermediate_node_parent p from to => (phrase_triple from p to)
     end.
 
   Definition node_to_phrase (s : SPPF_node) : (@phrase Tt triple):=
     match s with
     | mk_terminal_node t from to => [Ts (T t)]
     | mk_epsilon_node from to  => []
-    | mk_nonterminal_node v from to => [Vs (V (mkTriple from [Vs (V v)] to))]
-    | mk_intermediate_node p from to => [Vs (V (mkTriple from p to))]
+    | mk_nonterminal_node v from to => [Vs (V (var_triple from v to))]
+    | mk_intermediate_node p from to => [Vs (V (phrase_triple from p to))]
     end.
 
   Definition SPPF_rel_to_rule (r : SPPF_rel) : (@rule Tt triple) :=
     match r with
-    |  mk_rel p v n => let var := V (valid_parent_to_triple p v) in
+    |  mk_rel p v n => let var := V (valid_parent_to_triple v) in
                        match n with
                        | mk_packed_node1 n1 => R var (node_to_phrase n1)
                        | mk_packed_node2 n1 n2 => R var ((node_to_phrase n1) ++ (node_to_phrase n2))
@@ -66,7 +78,7 @@ Module Base.
 
 
   Theorem in_p_eq (p : SPPF_node) (is_p1 is_p2 : valid_parent p) :
-    (valid_parent_to_triple p is_p1 = valid_parent_to_triple p is_p2).
+    (valid_parent_to_triple is_p1 = valid_parent_to_triple is_p2).
   Proof.
     destruct is_p1.
     simpl.
@@ -93,81 +105,218 @@ Module Base.
     reflexivity.
   Qed.
 
-  Theorem in1 (t : Tt) (from to : nat) (p : SPPF_node) (is_p vp : valid_parent p) (sppf : SPPF) :
-    In (mk_rel p vp (mk_packed_node1 (mk_terminal_node t from to))) sppf ->
-    In (R (V (valid_parent_to_triple p is_p)) (to_phrase [T t])) (SPPF_to_grammar sppf).
+  Theorem in_conversion (sppf : SPPF) (r : SPPF_rel):
+  In r sppf -> In (SPPF_rel_to_rule r) (SPPF_to_grammar sppf).
   Proof.
-    intro H0.
     induction sppf.
     contradiction.
+    intro H0.
     destruct H0.
-    simpl.
     left.
     rewrite H.
-    simpl.
-    assert (Heq : (valid_parent_to_triple p vp) = (valid_parent_to_triple p is_p)).
-    apply in_p_eq.
-    rewrite Heq.
     reflexivity.
     right.
     apply IHsppf.
-    exact H.
+    auto.
   Qed.
 
-  Theorem in2 (from to : nat) (p : SPPF_node) (is_p vp : valid_parent p) (sppf : SPPF) :
-    In (mk_rel p vp (mk_packed_node1 (mk_epsilon_node from to))) sppf ->
-    In (R (V (valid_parent_to_triple p is_p)) (to_phrase [])) (SPPF_to_grammar sppf).
+  Theorem simpl_node_to_phrase (n : SPPF_node) (is_p : valid_parent n):
+       (node_to_phrase n) = [Vs (V (valid_parent_to_triple is_p))].
+  Proof.
+    destruct is_p.
+    simpl; reflexivity.
+    simpl; reflexivity.
+  Qed.
+
+  Theorem eq1 {A} (l: list A): l = [] ++ l ++ [].
+    simpl.
+    induction l.
+    reflexivity.
+    simpl.
+    rewrite <- IHl.
+    reflexivity.
+  Qed.
+
+
+  Theorem der_from_in (sppf : SPPF) (p : SPPF_node) (vp : valid_parent p) (ch1 : SPPF_node):
+
+  In (mk_rel vp (mk_packed_node1 ch1)) sppf ->
+  der (SPPF_to_grammar sppf) (V (valid_parent_to_triple vp)) (node_to_phrase ch1).
   Proof.
     intro H0.
-    induction sppf.
-    contradiction.
-    destruct H0.
-    left.
-    rewrite H.
-    simpl.
-    assert (Heq : (valid_parent_to_triple p vp) = (valid_parent_to_triple p is_p)).
-    apply in_p_eq.
-    rewrite Heq.
-    reflexivity.
-    right.
-    apply IHsppf.
-    exact H.
+    apply rDer.
+    apply (@in_conversion sppf (mk_rel vp (mk_packed_node1 ch1))).
+    apply H0.
   Qed.
+
+  Theorem to_phrase_conc {V0 T0} w1 w2: (@to_phrase V0 T0 (w1 ++ w2)) = (to_phrase w1 ++ to_phrase w2).
+    induction w1.
+    simpl.
+    reflexivity.
+    simpl.
+    rewrite IHw1.
+    reflexivity.
+  Qed.
+
+  Theorem der_cov1 (g : @grammar Tt triple) (A B: var) p0 p1
+          (der1 : der g A p0) (der2 :  der g B ([Vs A] ++ p1)): der g B (p0 ++ p1).
+
+   assert (eq1: forall(l1 l2: list (@symbol Tt triple)), l1 ++ l2 = [] ++ l1 ++ l2).
+    { intros.
+      simpl.
+      reflexivity.
+    }
+    rewrite (eq1 p0 p1).
+
+    apply replN with (B0 := A).
+
+    apply der2.
+
+    apply der1.
+  Qed.
+
+  Theorem der_cov2 (g : @grammar Tt triple) (A B: var) p0 p1
+          (der1 : der g A p1) (der2 :  der g B (p0 ++ [Vs A])): der g B (p0 ++ p1).
+
+   assert (eq1: forall(l1 l2: list (@symbol Tt triple)), l1 ++ l2 = l1 ++ l2 ++ []).
+    { intros.
+      rewrite app_nil_r.
+      reflexivity.
+    }
+    rewrite (eq1 p0 p1).
+
+    apply replN with (B0 := A).
+
+    apply der2.
+
+    apply der1.
+  Qed.
+
+
+  Theorem trains0 (sppf : SPPF) (n : SPPF_node) (w : word)
+           (d : (sppf_der sppf n w)) :
+    ext_der (SPPF_to_grammar sppf) (node_to_phrase n) (to_phrase w).
+  Proof.
+    induction d.
+    simpl.
+    apply refl.
+    simpl.
+    apply refl.
+    pose proof (simpl_node_to_phrase vp).
+    rewrite H0.
+    apply inDer.
+    remember (node_to_phrase ch1) as p1 in *.
+    remember (to_phrase w1) as p2 in *.
+    destruct IHd.
+    rewrite Heqp1.
+    apply der_from_in.
+    exact H.
+    rewrite (eq1 p0).
+    apply replN with (B := A).
+    rewrite <- (eq1 [Vs A]).
+    rewrite Heqp1.
+    apply  der_from_in.
+    exact H.
+    exact in_der.
+
+    rewrite (simpl_node_to_phrase vp).
+
+    rewrite (to_phrase_conc w1 w2).
+
+    pose proof (@in_conversion sppf (mk_rel vp (mk_packed_node2 ch1 ch2))) H.
+    clear H.
+
+    remember (node_to_phrase ch1) as p1 in *.
+    remember (to_phrase w1) as p2 in *.
+
+    destruct IHd1.
+
+    rewrite Heqp1.
+    clear d1 Heqp1 Heqp2.
+
+    remember (node_to_phrase ch2) as p1 in *.
+    remember (to_phrase w2) as p2 in *.
+
+    destruct IHd2.
+
+    rewrite Heqp1.
+
+    clear d2 Heqp1 Heqp2.
+
+    apply inDer .
+    apply rDer.
+    apply H0.
+
+    apply inDer.
+
+    apply der_cov2 with (A := A).
+    exact in_der.
+    rewrite Heqp1.
+
+    apply rDer.
+    exact H0.
+
+    remember (node_to_phrase ch2) as p1 in *.
+    remember (to_phrase w2) as p2 in *.
+
+    destruct IHd2.
+
+    apply inDer.
+
+    apply der_cov1 with (A := A).
+    exact in_der.
+    rewrite Heqp1.
+    rewrite Heqp0.
+
+    apply rDer.
+    exact H0.
+
+    apply inDer.
+
+    apply der_cov1 with (A := A).
+    exact in_der.
+    apply der_cov2 with (A := A0).
+    exact in_der0.
+    rewrite Heqp1.
+    rewrite Heqp0.
+
+    apply rDer.
+
+    exact H0.
+
+  Qed.
+
 
   Theorem trains1 (sppf : SPPF) (n : SPPF_node) (is_p : valid_parent n) (w : word)
            (d : (sppf_der sppf n w)) :
-    der (SPPF_to_grammar sppf) (V (valid_parent_to_triple n is_p)) (to_phrase w).
+     der (SPPF_to_grammar sppf) (V (valid_parent_to_triple is_p)) (to_phrase w).
   Proof.
-    induction d.
-    remember (mk_terminal_node t from to) as root in *.
-    destruct is_p; discriminate.
-    remember (mk_epsilon_node from to) as root in *.
-    destruct is_p; discriminate.
-    destruct ch1.
-    remember (mk_terminal_node t n n0) as root in *.
-    destruct d.
-    injection Heqroot.
-    clear Heqroot.
-    intro H0; rewrite H0 in *; clear H0.
-    intro H0; rewrite H0 in *; clear H0.
-    intro H0; rewrite H0 in *; clear H0.
+    pose proof trains0 d.
+    remember (node_to_phrase n) as p1 in *.
+    remember (to_phrase w) as p2 in *.
+    destruct H.
+    destruct is_p.
+    simpl in Heqp1.
+    rewrite  Heqp1 in Heqp2.
+    exfalso.
+    clear Heqp1 d p.
+    induction w.
+    discriminate.
+    discriminate.
+    exfalso.
+    rewrite  Heqp1 in Heqp2.
+    clear Heqp1 d p.
+    induction w.
+    discriminate.
+    discriminate.
 
-    apply rDer.
-    apply (in1 t n n0 p is_p vp).
-    exact H.
+    rewrite (simpl_node_to_phrase is_p) in Heqp1.
+    injection Heqp1.
+    intros.
 
-    apply rDer.
-
-    apply (in2 from to p is_p vp).
-    exact H.
-
-    rewrite -> Heqroot in IHd.
-    simpl IHd.
-    assert der (SPPF_to_grammar sppf) ((mkTriple n [Vs (V v)] n0)) (to_phrase w1).
-
-
-    apply IHd.
-
+    rewrite <- H.
+    exact in_der.
+  Qed.
 End Base.
 
 
